Lampe/Lampe/Hoare/SepTotal.lean
@@ -513,7 +513,7 @@ theorem lam_intro : STHoare p Γ ⟦⟧ (.lam argTps outTp lambdaBody)
   constructor
   intros
   simp_all only [SLP.true_star, SLP.star_assoc]
-  rename Ref => r
+  rename Address => r
   exists ⟨∅, Finmap.singleton r ⟨argTps, outTp, lambdaBody⟩⟩, st
   refine ⟨?_, ?_, ?_, ?_⟩
   . simp only [LawfulHeap.disjoint]
